src/Examples/Logging2/RefinementAlloc.v
@@ -3,6 +3,7 @@ Require Export CSL.Refinement CSL.NamedDestruct.
 Require Import AllocAPI ImplAlloc ExMach.WeakestPre ExMach.RefinementAdequacy.
 Require Import Logging2.Helpers.
 Require Import Equality.
+Require Import RefinementLog2.
 Set Default Proof Using "All".
 Unset Implicit Arguments.
 
@@ -45,6 +46,40 @@ Section refinement_triples.
       )
     )%I.
 
+  Definition heapT := @gen_heapG nat nat Σ nat_eq_dec nat_countable.
+  Definition memHeap := exmachG0.(@exm_mem_inG Σ).
+  Definition liftable (P : heapT -> iProp Σ) :=
+    (
+      ∀ (h1 : @gen_heapG nat nat Σ nat_eq_dec nat_countable),
+      P h1 -∗
+      ∃ m,
+      ([∗ map] a ↦ v ∈ m, a ↦[h1] v) ∗
+      ∀ (h2 : @gen_heapG nat nat Σ nat_eq_dec nat_countable),
+      ([∗ map] a ↦ v ∈ m, a ↦[h2] v) -∗
+      P h2
+    )%I.
+
+  Theorem lift_pred_ok : forall txn hT P,
+    (
+      ( txn_valid txn hT ∗
+        P memHeap ∗
+        liftable P
+      ) -∗
+      (
+        txn_valid txn hT ∗
+        P hT
+      )
+    )%I.
+  Proof.
+    iIntros (???) "(Htxn & Hp & Hliftable)".
+    unfold liftable.
+    iDestruct ("Hliftable" with "Hp") as (m) "[Hm Hp]".
+    iDestruct (lift_ok with "[$Htxn $Hm]") as "[Htxn Hm]".
+    iFrame.
+    iApply "Hp".
+    iFrame.
+  Qed.
+
   Axiom write_ok : forall s E txn a v v0 hT,
     (
       (
@@ -59,17 +94,18 @@ Section refinement_triples.
       }}
     )%I.
 
-  Axiom read_ok : forall s E txn a v hT,
+  Axiom read_ok : forall s E txn a v0 hT,
     (
       (
         txn_valid txn hT ∗
-        a ↦[hT] v
+        a ↦[hT] v0
       )
       -∗
       WP ImplAlloc.read txn a @ s; E {{
         v,
         txn_valid txn hT ∗
-        a ↦[hT] v
+        a ↦[hT] v0 ∗
+        ⌜ v = v0 ⌝
       }}
     )%I.
 
@@ -86,3 +122,214 @@ Section refinement_triples.
       }}
     )%I.
 
+  Theorem commit_pred_ok : forall s E txn P hT,
+    (
+      (
+        txn_valid txn hT ∗
+        liftable P ∗
+        P hT
+      )
+      -∗
+      WP ImplAlloc.commit txn @ s; E {{
+        r,
+        P memHeap
+      }}
+    )%I.
+  Proof.
+    iIntros (?????) "(Htxn & Hliftable & Hp)".
+    iDestruct ("Hliftable" with "Hp") as (m) "[Hm Hp]".
+    iDestruct (commit_ok with "[$Htxn $Hm]") as "Hcom".
+    iApply (wp_wand with "Hcom").
+    iIntros (?) "Hm".
+    iApply "Hp".
+    iFrame.
+  Qed.
+
+
+  Definition AllocState (h : heapT) (off : nat) (sz : nat) (freeset : gset nat) :=
+    (
+      ∃ freevals,
+      ⌜ length freevals = sz ⌝ ∗
+      ⌜ forall i, i < sz -> i ∈ freeset <-> freevals !! i = Some 0 ⌝ ∗
+      ([∗ list] i ↦ v ∈ freevals, (off+i) ↦[h] v)
+    )%I.
+
+  Definition AllocInv (freeset : gset nat) (h : heapT) :=
+    ( ∃ sz,
+      allocator ↦[h] sz ∗
+      AllocState h (allocator+1) sz freeset
+    )%I.
+
+  Theorem alloc_below_ok : forall s E txn off n hT sz fs,
+    (
+      (
+        txn_valid txn hT ∗
+        AllocState hT off sz fs ∗
+        ⌜ n <= sz ⌝
+      )
+      -∗
+      WP ImplAlloc.alloc_below txn off n @ s; E {{
+        r,
+        txn_valid txn hT ∗
+        match r with
+        | None => AllocState hT off sz fs
+        | Some a => AllocState hT off sz (fs ∖ {[a]})
+        end
+      }}
+    )%I.
+  Proof.
+    intros.
+    iIntros "(Htxn & Has & Hp)".
+    iDestruct "Has" as (freevals) "[%[%Has]]".
+    iInduction n as [|n] "IH"; simpl.
+    - wp_ret. iFrame.
+      iExists _. iFrame. iPureIntro. intuition.
+    - iPure "Hp" as Hp.
+      edestruct @lookup_lt_is_Some_2 with (i := n) (l := freevals). lia.
+      destruct (decide (x = 0)).
+      + iDestruct (big_sepL_insert_acc with "Has") as "[Hn Hother]". eauto.
+        wp_bind.
+        iDestruct (read_ok with "[$Htxn $Hn]") as "Hwp_read".
+        iApply (wp_wand with "Hwp_read").
+        iIntros (?) "[Htxn [Hn%]]"; subst.
+        iDestruct (write_ok with "[$Htxn $Hn]") as "Hwp_write".
+        wp_bind.
+        iApply (wp_wand with "Hwp_write").
+        iIntros (?) "[Htxn Hn]".
+        wp_ret. iFrame.
+        iDestruct ("Hother" with "Hn") as "Hfv".
+        iExists _. iFrame.
+        iPureIntro. intuition. rewrite insert_length. auto.
+        * destruct (decide (i = n)); subst.
+          { admit. }
+          { admit. }
+        * destruct (decide (i = n)); subst.
+          { admit. }
+          { admit. }
+      + iDestruct (big_sepL_lookup_acc with "Has") as "[Hn Hother]". eauto.
+        wp_bind.
+        iDestruct (read_ok with "[$Htxn $Hn]") as "Hwp_read".
+        iApply (wp_wand with "Hwp_read").
+        iIntros (?) "[Htxn [Hn%]]"; subst.
+        destruct (decide (x = 0)); try congruence.
+        iDestruct ("Hother" with "Hn") as "Hfv".
+        iApply ("IH" with "[$Htxn] [$Hfv]").
+        iPureIntro. lia.
+  Admitted.
+
+  Theorem alloc_ok : forall s E txn hT fs,
+    (
+      (
+        txn_valid txn hT ∗
+        AllocInv fs hT
+      )
+      -∗
+      WP ImplAlloc.alloc txn @ s; E {{
+        r,
+        txn_valid txn hT ∗
+        match r with
+        | None => AllocInv fs hT
+        | Some a => AllocInv (fs ∖ {[a]}) hT
+        end
+      }}
+    )%I.
+  Proof.
+    intros.
+    iIntros "[Htxn Hinv]".
+    iDestruct "Hinv" as (sz) "[Hsz Has]".
+    wp_bind.
+    iDestruct (read_ok with "[$Htxn $Hsz]") as "Hwp_read".
+    iApply (wp_wand with "Hwp_read").
+    iIntros (?) "[Htxn [Hsz%]]"; subst.
+    iDestruct (alloc_below_ok with "[$Htxn $Has]") as "Hwp_allow_below".
+    2: iApply (wp_wand with "Hwp_allow_below").
+    iPureIntro. lia.
+    iIntros (?) "[Htxn Hret]".
+    iFrame.
+    destruct a.
+    - iExists _. iFrame.
+    - iExists _. iFrame.
+  Qed.
+
+  Definition mem_lock := 0.
+  Definition aN : namespace := (nroot.@"alloc_lock").
+  Definition BigInv :=
+    (
+      ∃ γlock,
+      is_lock aN γlock mem_lock (∃ AS, AllocInv AS memHeap)
+    )%I.
+
+  Definition alloc_and_commit :=
+    (
+      txn <- begin;
+      _ <- ExMachAPI.lock mem_lock;
+      r <- alloc txn;
+      _ <- commit txn;
+      _ <- ExMachAPI.unlock mem_lock;
+      Ret r
+    )%proc.
+
+  Theorem AllocInv_liftable : forall s,
+    liftable (AllocInv s).
+  Proof.
+    unfold liftable.
+    intros.
+    iIntros (?) "H".
+    iDestruct "H" as (sz) "[Hsz Has]".
+  Admitted.
+
+  Theorem alloc_and_commit_ok :
+    (
+      (
+        BigInv
+      )
+      -∗
+      WP alloc_and_commit {{
+        r,
+        BigInv
+      }}
+    )%I.
+  Proof.
+    intros.
+    iIntros "Hinv".
+    iDestruct "Hinv" as (l) "#Hinv".
+
+    iDestruct (begin_ok) as "Hwp_begin".
+    wp_bind.
+    iApply (wp_wand with "Hwp_begin").
+    iIntros (?) "Htxn".
+    iDestruct "Htxn" as (txn) "Htxn".
+
+    wp_bind.
+    wp_lock "[Hlocked Hopen]".
+    iDestruct "Hopen" as (AS) "Hopen".
+
+    iPoseProof AllocInv_liftable as "Hliftable".
+    iDestruct (lift_pred_ok with "[$Htxn Hopen $Hliftable]") as "[Htxn Hopen]".
+    iFrame.
+
+    iDestruct (alloc_ok with "[$Htxn $Hopen]") as "Hwp_alloc".
+    wp_bind.
+    iApply (wp_wand with "Hwp_alloc").
+    iIntros (?) "[Htxn Hres]".
+
+    destruct a0.
+    - iPoseProof AllocInv_liftable as "Hliftable2".
+      iDestruct (commit_pred_ok with "[$Htxn $Hliftable2 $Hres]") as "Hwp_commit".
+      wp_bind.
+      iApply (wp_wand with "Hwp_commit").
+      iIntros (?) "Hopen".
+
+      wp_unlock "[Hopen]". iExists _. iFrame.
+      wp_ret.
+      iExists _. iApply "Hinv".
+
+    - iDestruct (commit_pred_ok with "[$Htxn $Hliftable $Hres]") as "Hwp_commit".
+      wp_bind.
+      iApply (wp_wand with "Hwp_commit").
+      iIntros (?) "Hopen".
+
+      wp_unlock "[Hopen]". iExists _. iFrame.
+      wp_ret.
+      iExists _. iApply "Hinv".
+  Qed.
